src/tls/KeySchedule.fst
@@ -43,7 +43,7 @@ open HSCrypto
 
 //abstract type ms = b:bytes{length b == 48}
 // ADL: Unsound!!
-type ms = PRF.masterSecret
+type ms = bytes
 type pms = PMS.pms 
 // Requires meta-argument to show that pms is not used concretely in other modules
 
@@ -56,7 +56,7 @@ type pms = PMS.pms
 // algId: id -> aeAlg) and its concrete definition may
 // be used to prove that StatefulLHAE.gen is not called
 // twice with the same id
-type id = TLSInfo.id
+//type id = TLSInfo.id
 
 // (in TLSInfo.fst)
 // type id = {
@@ -135,71 +135,74 @@ type ks =
 **)
 
 // Agility parameters, extend as needed
-type ks_alpha = pv:protocolVersion * cs:cipherSuite * ems:bool
+// may be moved to TLSInfo for joint idealization with Handshake
+type ks_alpha = pv:protocolVersion * cs:cipherSuite * nego:negotiatedExtensions
 
 // Internal KS state, now with ad-hoc parameters
-type kx_state =
+type ks_state =
 | KS_C_Init
-| KS_C_12_Resume_CH of cr:random * si:sessionInfo * msId:TLSInfo.msId * ms:ms
-| KS_C_12_Full_CH of cr:random
-// Wait for session hash to compute EMS
-| KS_C_12_Full_SH_EMS of cr:random * sr:random * alpha:ks_alpha * id:TLSInfo.pmsId * pms:bytes
-// No EMS, master secret is computed immediately
-| KS_C_12_Full_SH_MS of cr:random * sr:random * alpha:ks_alpha * id:TLSInfo.msId * ms:ms
-| KS_C_12_Resume_SH of cr:random * sr:random * alpha:ks_alpha * si:sessionInfo * id:TLSInfo.msId * ms:ms
+| KS_C_12_Resume_CH: cr:random -> si:sessionInfo -> msId:TLSInfo.msId -> ms:ms -> ks_state
+| KS_C_12_Full_CH: cr:random -> ks_state
+| KS_C_12_wait_MS: csr:csRands -> alpha:ks_alpha -> id:TLSInfo.pmsId -> pms:bytes -> ks_state
+| KS_12_has_MS: r:role -> csr:csRands -> alpha:ks_alpha -> id:TLSInfo.msId -> ms:ms -> ks_state
 | KS_S_Init
+| KS_Done
 
 type ks =
 | KS: #region:rid -> cfg:config -> state:rref region ks_state -> ks
 
 // Create a fresh key schedule instance
 // We expect this to be called when the Handshake instance is created
-let create #region:rid cfg:config r:role
-  -> ST ks
-  (requires fun h -> r<>root)
-  (ensures fun h0 r h1 -> 
-    let KS ks_region cfg state = r in
+val create: #rid:rid -> config -> role -> ST ks
+  (requires fun h -> rid<>root)
+  (ensures fun h0 r h1 ->
+    let KS #ks_region cfg state = r in
     fresh_region ks_region h0 h1
-    /\ extends ks_region region) =
-  ST.recall_region region;
-  let ks_region = new_region region in 
+    /\ extends ks_region rid)
+
+let create #rid cfg r =
+  ST.recall_region rid;
+  let ks_region = new_region rid in 
   let istate = match r with | Client -> KS_C_Init | Server -> KS_S_Init in
-  KS region cfg (ralloc ks_region istate)
+  KS #ks_region cfg (ralloc ks_region istate)
 
 // Called before sending client hello
 // (the external style of resumption may become internal to protect ms abstraction)
-let ks_client_init_12 ks:ks
-  -> ST (cr:random * si:option sessionInfo)
-  (requires fun h0 -> sel h0 (KX.state ks) = KS_C_Init)
-  (ensures fun h0 r h1 -> True) =
-  let cr = Nonces.mkHelloRandom () in
-  let osi, ns = match cfg.resuming with
-    | None -> None, KS_C_12_Full_CH cr
-    | Some shard ->
-      (match DB.lookup shard with
-      | Some (si, msId, ms) -> Some si, KS_C_12_Resume_CH cr si msId ms in
-      | None -> None, KS_C_12_Full_CH cr) in
+val ks_client_init_12: ks:ks -> ST (random * option sessionInfo)
+  (requires fun h0 -> sel h0 (KS.state ks) = KS_C_Init)
+  (ensures fun h0 r h1 -> True)
+
+// TODO resumption support
+let ks_client_init_12 ks =
+  let cr = Nonce.mkHelloRandom () in
+  let osi, ns = None, (KS_C_12_Full_CH cr) in
+//    match cfg.resuming with
+//    | None -> None, (KS_C_12_Full_CH cr)
+//    | Some shard ->
+//      (match DB.lookup shard with TODO
+//      | Some (si, msId, ms) -> (Some si), (KS_C_12_Resume_CH cr si msId ms)
+//      | None -> None, (KS_C_12_Full_CH cr)) in
   (KS.state ks) := ns;
   cr, osi
 
 // Called after receiving server hello; server accepts resumption proposal
 // This function only checks the agility paramaters compared to the resumed sessionInfo
 // and returns to the handshake whether the resumption is permissible
-let ks_client_12_resume_sh ks:ks sr:random alpha:ks_alpha
-  -> ST cvd:bytes
+val ks_client_12_resume: ks:ks -> random -> alpha:ks_alpha -> ST unit
   (requires fun h0 ->
-    let kss = sel h0 (KX.state ks) in
-    let (pv, cs, ems) = alpha in
+    let kss = sel h0 (KS.state ks) in
+    let (pv, cs, nego) = alpha in
     is_KS_C_12_Resume_CH kss
     /\ (let si = KS_C_12_Resume_CH.si kss in
       si.protocol_version = pv /\ si.cipher_suite = cs
-      /\ (is_Some si.session_hash <==> ems)))
-  (ensures fun h0 cvd h1 -> True) =
-  let KS region cfg st = ks in
+      /\ (si.extensions.ne_extended_ms <==> nego.ne_extended_ms)))
+  (ensures fun h0 cvd h1 -> True)
+
+let ks_client_12_resume ks sr alpha =
+  let KS #region cfg st = ks in
   let KS_C_12_Resume_CH cr si msId ms = !st in
-  st := KS_C_12_Resume_SH cr sr si ms;
-  let (pv, cs, ems) = alpha in
-  
+  let csr = cr @| sr in
+  st := KS_12_has_MS Client csr alpha msId ms
 
 // The two functions below are similar but we decide not to factor them because:
 //   1. they use different arguemtns
@@ -207,85 +210,111 @@ let ks_client_12_resume_sh ks:ks sr:random alpha:ks_alpha
 //   3. they are called at different locations
 
 // Called by Hanshake when DH key echange is negotiated
-let ks_client_12_full_sh_dh ks:ks sr:random alpha:ks_alpha dhp:CommonDH.params peer_share:CommonDH.share 
-  -> ST CommonDH.share
+val ks_client_12_full_dh: ks:ks -> random -> ks_alpha -> CommonDH.params -> peer_share:CommonDH.key -> ST CommonDH.key
   (requires fun h0 ->
-    let st = sel h0 (KX.state ks) in
+    let st = sel h0 (KS.state ks) in
     is_KS_C_12_Full_CH st \/ is_KS_C_12_Resume_CH st)
-  (ensures fun h0 r h1 ->
-    True //modifies (Set.singleton r) h0 h1
-    /\ CommonDH.group_of r = CommonDH.group_of peer_share) =
-  let KS region cfg st = ks in
-  let (pv, cs, ems) = alpha in
-  let cr = match !st with | KS_C_12_Full_CH cr -> cr | KS_C_12_Resume_CH cr _ _ -> cr in
+  (ensures fun h0 r h1 -> True)
+
+let ks_client_12_full_dh ks sr alpha dhp peer_share =
+  let KS #region cfg st = ks in
+  let (pv, cs, nego) = alpha in
+  let cr = match !st with
+    | KS_C_12_Full_CH cr -> cr
+    | KS_C_12_Resume_CH cr _ _ _ -> cr in
+  let csr = cr @| sr in
   let our_share, pmsb = CommonDH.dh_responder peer_share in
-  let dhpms = PMS.DHPMS(dhp, our_share, peer_share, pmsb) in
+  let dhpms = PMS.DHPMS(dhp, our_share, peer_share, PMS.ConcreteDHPMS(pmsb)) in
   let dhpmsId = TLSInfo.SomePmsId(dhpms) in
   let ns = 
-    if ems then KS_C_12_Full_SH_EMS cr sr dhpmsId pmsb
+    if nego.ne_extended_ms then
+      KS_C_12_wait_MS csr alpha dhpmsId pmsb
     else
-      let csr = cr @| sr in
-      let ms = TLSPRF.extract (kefAlg alpha) pmsb csr 48 in
-      let msId = StandardMS dhpms csr (kefAlg alpha) in
-      KS_C_12_Full_SH_MS msId ms in
-  st := ns; out_share
+      let kef = kefAlg pv cs true in
+      let ms = TLSPRF.extract kef pmsb csr 48 in
+      let msId = StandardMS dhpmsId csr kef in
+      KS_12_has_MS Client csr alpha msId ms in
+  st := ns; our_share
 
 // Called by Handshake after server hello when a full RSA key exchange is negotiated
-let ks_client_12_full_sh_rsa ks:ks sr:random alpha:ks_alpha pk:RSAKey.pk
-  -> ST encryptedPMS:bytes
+val ks_client_12_full_rsa: ks:ks -> random -> ks_alpha -> RSAKey.pk -> ST bytes
   (requires fun h0 ->
-    let st = sel h0 (KX.state ks) in
+    let st = sel h0 (KS.state ks) in
     is_KS_C_12_Full_CH st \/ is_KS_C_12_Resume_CH st)
-  (ensures fun h0 r h1 -> True) =
-  let KS region cfg st = ks in
-  let (pv, cs, ems) = alpha in
-  let cr = match !st with | KS_C_12_Full_CH cr -> cr | KS_C_12_Resume_CH cr _ _ -> cr in
+  (ensures fun h0 r h1 -> True)
+
+let ks_client_12_full_rsa ks sr alpha pk =
+  let KS #region cfg st = ks in
+  let (pv, cs, nego) = alpha in
+  let cr = match !st with
+    | KS_C_12_Full_CH cr -> cr
+    | KS_C_12_Resume_CH cr _ _ _ -> cr in
+  let csr = cr @| sr in
   let rsapms = PMS.genRSA pk pv in
-  let encrypted = RSA.encrypt pk pv rsapms in
   let pmsb = PMS.leakRSA pk pv rsapms in
+  let encrypted = CoreCrypto.rsa_encrypt (RSAKey.repr_of_rsapkey pk) CoreCrypto.Pad_PKCS1 pmsb in
   let rsapmsId = TLSInfo.SomePmsId(PMS.RSAPMS(pk, pv, rsapms)) in
   let ns =
-    if ems then KS_C_12_Full_SH_EMS cr sr pk rsapmsId pmsb
+    if nego.ne_extended_ms then
+      KS_C_12_wait_MS csr alpha rsapmsId pmsb
     else
-      let csr = cr @| sr in
-      let ms = TLSPRF.extract (kefAlg alpha) pmsb csr 48 in
-      let msId = StandardMS rsapms csr (kefAlg alpha) in
-      KS_C_12_Full_SH_MS msId ms in
+      let kef = kefAlg pv cs true in
+      let ms = TLSPRF.extract kef pmsb csr 48 in
+      let msId = StandardMS rsapmsId csr kef in
+      KS_12_has_MS Client csr alpha msId ms in
   st := ns; encrypted
 
 // This MUST be called by handshake as soon as session hash is available if EMS was negotiated
-let ks_client_12_set_session_hash ks:ks session_hash:bytes
-  -> ST unit
+val ks_client_12_set_session_hash: ks:ks -> bytes -> ST unit
   (requires fun h0 ->
-    let st = sel h0 (KX.state ks) in
-    is_KS_C_12_Full_SH_EMS st)
-  (ensures fun h0 r h1 ->
-    True) =
-  let KS region cfg st = ks in
-  let KS_C_12_Full_SH_EMS cr, sr, pmsid, pms = !st in
-  let ca = kefAlgExtended si in
-  let ms = TLSPRF.extract ca pms session_hash 48 in
-  let msId = ExtendedMS id session_hash ca in
-  st := KS_C_12_Full_SH_MS msId ms
+    let st = sel h0 (KS.state ks) in
+    is_KS_C_12_wait_MS st)
+  (ensures fun h0 r h1 -> True)
+
+let ks_client_12_set_session_hash ks session_hash =
+  let KS #region cfg st = ks in
+  let KS_C_12_wait_MS csr alpha pmsid pms = !st in
+  let (pv, cs, nego) = alpha in
+  let kef = kefAlg pv cs nego.ne_extended_ms in
+  let ms = TLSPRF.extract kef pms session_hash 48 in
+  let msId = ExtendedMS pmsid session_hash kef in
+  st := KS_12_has_MS Client csr alpha msId ms
 
 // *********************************************************************************
 //  All functions below assume that the MS is already computed (and thus they are
-//  shared accross role, key exchange, handshake mode...
+//  shared accross role, key exchange, handshake mode...)
 // *********************************************************************************
 
-let ks_12_get_finished ks:ks log:bytes
-  -> ST bytes
+val ks_12_finished: ks:ks -> bytes -> ST (vd:bytes * wk:bytes * wiv:bytes * rk:bytes * riv:bytes)
   (requires fun h0 ->
-    let st = sel h0 (KX.state ks) in
-    is_KS_C_12_Full_SH_MS st \/ is_KS_C_12_Full_Resume_SH st)
-  (ensures fun h0 r h1 ->
-    True) =
-  let KS region cfg st = ks in
-  let ms = match kss with
-    | KS_C_12_Full_SH_MS of id:TLSInfo.msId * ms:ms
-    | KS_C_12_Full_SH 
-| KS_C_12_Resume_SH of cr:random * sr:random * si:sessionInfo * ms:ms
-  TLSPRF.verifyData (pv,cs) ms Client log
+    let st = sel h0 (KS.state ks) in
+    is_KS_12_has_MS st)
+  (ensures fun h0 r h1 -> True)
+
+let ks_12_finished ks log =
+  let KS #region cfg st = ks in
+  let KS_12_has_MS role csr alpha msId ms = !st in
+  let (pv, cs, nego) = alpha in
+  let vd = TLSPRF.verifyData (pv,cs) ms role log in
+  let ae_id = {
+    msId = msId;
+    kdfAlg = kdfAlg pv cs;
+    pv = pv;
+    aeAlg = get_aeAlg cs;
+    csrConn = csr;
+    ext = nego;
+    writer = role
+  } in
+  let expand = TLSPRF.kdf ae_id.kdfAlg ms csr 40 in
+  let k1, expand = split expand 16 in
+  let k2, expand = split expand 16 in
+  let iv1, iv2 = split expand 4 in
+  let wk, wiv, rk, riv =
+    match role with
+    | Client -> k1, iv1, k2, iv2
+    | Server -> k2, iv2, k1, iv1 in
+  st := KS_Done; // Destroy MS
+  (vd, wk, wiv, rk, riv)
 
 
 (* MK: older experiment with Antoine
